Ported revisions 8448:8497 from HOL to HOL-Omega. This is to keep HOL-Omega current with the latest HOL developments.

developers/mlsysinfo.sml
@@ -1,0 +1,12 @@
+let
+  fun fact n acc = if n <= 1 then acc else fact (n - 1) (n * acc)
+in
+  fact 21 1;
+  use "polysysinfo.sml"
+     handle e =>
+        if String.isPrefix "Io" (exnMessage e) then
+          print "\n\n** You must do\n     poly < mlsysinfo.sml\n\
+                \** from the HOL/developers directory\n\n"
+        else ()
+end
+handle Overflow => use "mosmlsysinfo.sml";
