developers/polysysinfo.sml
@@ -1,0 +1,9 @@
+val _ = PolyML.print_depth 0;
+val version_string_w1 =
+    hd (String.tokens Char.isSpace PolyML.Compiler.compilerVersion)
+    handle Empty => ""
+val compiler_number =
+    Real.floor (100.0 * valOf (Real.fromString version_string_w1))
+    handle Option => 0
+val _ = print ("\nMLSYSTEM = poly"^Int.toString compiler_number^"\n");
+
