examples/acl2/tests/gold/defund-test.lisp
@@ -1,5 +1,20 @@
+; NOTE: Forms below are not evaluated when translating to ML.
 (IN-PACKAGE "ACL2")
 
 (DEFUN FOO (X) X)
 
 (DEFUN BAR (X) X)
+
+(MUTUAL-RECURSION (DEFUN EVENLP (X)
+                         (IF (CONSP X) (ODDLP (CDR X)) 'T))
+                  (DEFUN ODDLP (X)
+                         (IF (CONSP X) (EVENLP (CDR X)) 'NIL)))
+
+(MUTUAL-RECURSION (DEFUN EVENLP2 (X)
+                         (PROG2$ (THROW-NONEXEC-ERROR 'EVENLP2
+                                                      (CONS X 'NIL))
+                                 (IF (CONSP X) (ODDLP2 (CDR X)) 'T)))
+                  (DEFUN ODDLP2 (X)
+                         (PROG2$ (THROW-NONEXEC-ERROR 'ODDLP2
+                                                      (CONS X 'NIL))
+                                 (IF (CONSP X) (EVENLP2 (CDR X)) 'NIL))))
