examples/acl2/tests/gold/pkg-test.ml
@@ -1,12 +1,5 @@
 val _ = sexp.acl2_list_ref := [
 
-(mkpair (mksym "ACL2" "DEFPKG") (mkpair (mk_chars_str (chars_to_string (cons 
-77 (cons 89 (cons 45 (cons 80 (cons 75 (cons 71 nil)))))))) (mkpair (mkpair (
-mksym "COMMON-LISP" "QUOTE") (mkpair (mkpair (mksym "COMMON-LISP" "CONS") (
-mkpair (mksym "COMMON-LISP" "DEFUN") (mksym "COMMON-LISP" "NIL"))) (mksym 
-"COMMON-LISP" "NIL"))) (mksym "COMMON-LISP" "NIL"))))
-,
-
 (mkpair (mksym "COMMON-LISP" "DEFUN") (mkpair (mksym "MY-PKG" "F1") (mkpair (
 mkpair (mksym "MY-PKG" "X") (mksym "COMMON-LISP" "NIL")) (mkpair (mkpair (
 mksym "COMMON-LISP" "CONS") (mkpair (mksym "MY-PKG" "X") (mkpair (mksym 
@@ -15,7 +8,7 @@ mksym "COMMON-LISP" "CONS") (mkpair (mksym "MY-PKG" "X") (mkpair (mksym
 
 (mkpair (mksym "COMMON-LISP" "DEFUN") (mkpair (mksym "MY-PKG" "F2") (mkpair (
 mkpair (mksym "MY-PKG" "X") (mksym "COMMON-LISP" "NIL")) (mkpair (mkpair (
-mksym "MY-PKG" "BINARY-APPEND") (mkpair (mksym "MY-PKG" "X") (mkpair (mksym 
+mksym "ACL2" "BINARY-APPEND") (mkpair (mksym "MY-PKG" "X") (mkpair (mksym 
 "MY-PKG" "X") (mksym "COMMON-LISP" "NIL")))) (mksym "COMMON-LISP" "NIL")))))
 
 ];
