examples/acl2/tests/gold/summary.ml
@@ -1,10 +1,5 @@
 val _ = sexp.acl2_list_ref := [
 
-(mkpair (mksym "ACL2" "INCLUDE-BOOK") (mkpair (mk_chars_str (chars_to_string (
-cons 114 (cons 101 (cons 99 (cons 111 (cons 114 (cons 100 (cons 115 nil))))))))) (
-mksym "COMMON-LISP" "NIL")))
-,
-
 (mkpair (mksym "COMMON-LISP" "DEFUN") (mkpair (mksym "ACL2" "UPDATE-MACRO") (
 mkpair (mkpair (mksym "ACL2" "UPDS") (mkpair (mksym "ACL2" "RESULT") (mksym 
 "COMMON-LISP" "NIL"))) (mkpair (mkpair (mksym "COMMON-LISP" "IF") (mkpair (
