examples/ARM/experimental/lpc_devicesScript.sml
@@ -1,0 +1,175 @@
+
+open HolKernel boolLib bossLib Parse;
+open wordsTheory pred_setTheory;
+
+open armTheory arm_stepTheory lpc_uartTheory;
+
+val _ = new_theory "lpc_devices";
+
+
+(* We define the type of a generic device *)
+
+val _ = type_abbrev ("device",``: 
+   (* memory addresses that belong to this device, dependent on internal state of type 'a *)
+   ('a -> word32 set) #     
+   (* if core executes a memory read, it sees the following data *)
+   ('a -> word32 -> word8) # 
+   (* the next state relation for the devive  *)
+   (num -> memory_access list -> 'a -> 'a -> bool) #
+   (* an invariant that mst be true for this devie to make sense *)
+   (num # 'a -> bool)``); 
+
+
+(* Devices can be composed *)
+
+val ACCESS_ADDRESS_def = Define `
+  (ACCESS_ADDRESS (MEM_READ w) = w) /\
+  (ACCESS_ADDRESS (MEM_WRITE w v) = w)`;
+
+val FILTER_ACCESSES_def = Define `
+  FILTER_ACCESSES d = FILTER (\x. (ACCESS_ADDRESS x) IN d)`;
+
+val COMPOSE_DEVICES_def = Define `
+  COMPOSE_DEVICES ((a1,m1,n1,i1):'a device) ((a2,m2,n2,i2):'b device) =
+     (* the combined addresses are the UNION of the two address sets *)
+    ((\(x,y). a1 x UNION a2 y),
+     (* memory reads are directed according to address ownership *)
+     (\(x,y) addr. if addr IN a1 x then m1 x addr else m2 y addr),
+     (* the combined next state relation filters memory accesses so that 
+        respective devices only see relevant memoy accesses *)
+     (\t l (x1,y1) (x2,y2). n1 t (FILTER_ACCESSES (a1 x1) l) x1 x2 /\ 
+                            n2 t (FILTER_ACCESSES (a2 y1) l) y1 y2),
+     (* the invariant is the conjunction of part invariants and the condition 
+        that the space used by these devices does not overlap. *)
+     (\(t,(x,y)). DISJOINT (a1 x) (a2 y) /\ i1 (t,x) /\ i2 (t,y))):('a # 'b) device`
+
+
+(* The most basic device: the EMPTY_DEVICE *)
+
+val EMPTY_DEVICE_def = Define `
+  (EMPTY_DEVICE:unit device) = ((\x. {}),(\x y. ARB),(\n l x y. T),(\x. T))`;
+
+
+(* RAM device *)
+
+val domain_def = Define `domain r = { a | ~(r a = NONE) }`;
+
+val UPDATE_RAM_def = Define `
+  (UPDATE_RAM [] ram = ram) /\
+  (UPDATE_RAM ((MEM_READ w)::xs) ram = UPDATE_RAM xs ram) /\ 
+  (UPDATE_RAM ((MEM_WRITE w v)::xs) ram = UPDATE_RAM xs (\a. if a = w then SOME v else ram a))`;
+
+val RAM_NEXT_def = Define `
+  RAM_NEXT (t:num) l (r1:word32 -> word8 option) r2 = (r2 = UPDATE_RAM l r1)`;
+
+val RAM_DEVICE_def = Define `
+  (RAM_DEVICE:(word32 -> word8 option) device) =
+    (domain, (\m addr. THE (m addr)), RAM_NEXT, (\x. T))`;
+
+
+(* ROM device - disallows write accesses *)
+
+val IS_WRITE_def = Define `
+  (IS_WRITE (MEM_READ w) = F) /\
+  (IS_WRITE (MEM_WRITE w v) = T)`;
+
+val ROM_NEXT_def = Define `
+  ROM_NEXT (t:num) l r1 r2 = (r2 = r1) /\ (FILTER IS_WRITE l = [])`;
+
+val ROM_DEVICE_def = Define `
+  (ROM_DEVICE:(word32 -> word8 option) device) =
+    (domain, (\m addr. THE (m addr)), ROM_NEXT, (\x. T))`;
+
+
+(* UART0 device *)
+
+val UART0_DEVICE_def = Define `
+  (UART0_DEVICE:uart0_state device) =
+    ((\x. UART0_addresses), UART0_read, UART0_NEXT, \(x,y). uart0_ok x y)`;
+
+
+(* The collection of all peripherals *)
+
+val ALL_PERIPHERALS_def = Define `
+  ALL_PERIPHERALS = 
+   (COMPOSE_DEVICES (ROM_DEVICE) 
+   (COMPOSE_DEVICES (RAM_DEVICE) 
+   (COMPOSE_DEVICES (UART0_DEVICE) 
+                    (EMPTY_DEVICE))))`;
+
+val PERIPHERALS_NEXT_def = Define `
+  PERIPHERALS_NEXT = 
+    let (addresses,mem,next,inv) = ALL_PERIPHERALS in 
+      \l (t1,x) (t2,y). 
+        next t1 l x y /\ (t2 = t1 + 1) /\ 
+        (FILTER_ACCESSES (UNIV DIFF addresses x) l = [])`;
+
+val PERIPHERALS_OK_def = Define `
+  PERIPHERALS_OK = 
+    let (addresses,mem,next,inv) = ALL_PERIPHERALS in inv`;
+
+val MEMORY_IMAGE_def = Define `
+  MEMORY_IMAGE (t:num,s) = 
+    let (addresses,mem,next,inv) = ALL_PERIPHERALS in mem s`;
+
+val PENDING_INTERRUPT_def = Define `
+  PENDING_INTERRUPT p1 = NoInterrupt`;
+
+val peripherals_type = 
+  ``PERIPHERALS_NEXT`` |> type_of |> dest_type |> snd |> el 2
+                                  |> dest_type |> snd |> el 1
+                                   
+val _ = type_abbrev ("peripherals", peripherals_type)
+
+val PER_READ_ROM_def = Define `PER_READ_ROM ((t,x,y):peripherals) a = THE (x a)`;
+val PER_READ_RAM_def = Define `PER_READ_RAM ((t,x,y,z):peripherals) a = THE (y a)`;
+val PER_READ_UART_def = Define `PER_READ_UART ((t,x,y,u,z):peripherals) a = u`;
+
+
+(* The overall next-state relation *)
+
+val LOAD_IMAGE_def = Define `
+  LOAD_IMAGE (s:arm_state) m = s with <|memory := m; accesses := []|>`;
+
+val LPC_NEXT_def = Define `
+  LPC_NEXT (s1,p1) (s2,p2) =
+    (ARM_NEXT (PENDING_INTERRUPT p1) 
+              (LOAD_IMAGE s1 (MEMORY_IMAGE p1)) = SOME s2) /\ 
+    PERIPHERALS_NEXT s2.accesses p1 p2`;
+
+
+(* Theorems *)
+
+val domain_UPDATE_RAM = prove(
+  ``!l p. (domain (UPDATE_RAM
+            (FILTER (\x. ACCESS_ADDRESS x IN domain p) l) p) = domain p)``,
+  SIMP_TAC std_ss [GSPECIFICATION] THEN Induct_on `l`
+  THEN SIMP_TAC std_ss [UPDATE_RAM_def,listTheory.FILTER]
+  THEN Cases_on `h` THEN SIMP_TAC std_ss [ACCESS_ADDRESS_def]
+  THEN REPEAT STRIP_TAC THEN Cases_on `c IN domain p` THEN ASM_SIMP_TAC std_ss []
+  THEN ASM_SIMP_TAC std_ss [UPDATE_RAM_def]
+  THEN `domain p = domain (\a. if a = c then SOME c0 else p a)` by 
+   (FULL_SIMP_TAC std_ss [domain_def,GSPECIFICATION,EXTENSION]
+    THEN REPEAT STRIP_TAC THEN Cases_on `x = c` THEN ASM_SIMP_TAC std_ss []) 
+  THEN ASM_SIMP_TAC std_ss []);
+
+val IMP_PERIPHERALS_OK = store_thm("IMP_PERIPHERALS_OK",
+  ``!p1 p2 l.
+      PERIPHERALS_OK p1 /\ PERIPHERALS_NEXT l p1 p2 ==>
+      PERIPHERALS_OK p2``,
+  SIMP_TAC std_ss [PERIPHERALS_OK_def,ALL_PERIPHERALS_def,UART0_DEVICE_def,
+    COMPOSE_DEVICES_def,ROM_DEVICE_def,RAM_DEVICE_def,EMPTY_DEVICE_def,
+    pairTheory.FORALL_PROD,LET_DEF,PERIPHERALS_NEXT_def,FILTER_ACCESSES_def,
+    listTheory.FILTER,ROM_NEXT_def,RAM_NEXT_def,UPDATE_RAM_def]
+  THEN SIMP_TAC std_ss [domain_UPDATE_RAM,UART0_NEXT_def]);
+
+val PERIPHERALS_NEXT_EXISTS = store_thm("PERIPHERALS_NEXT_EXISTS",
+  ``!p1. PERIPHERALS_OK p1 ==> ?p2. PERIPHERALS_NEXT [] p1 p2``,
+  SIMP_TAC std_ss [PERIPHERALS_OK_def,ALL_PERIPHERALS_def,UART0_DEVICE_def,
+    COMPOSE_DEVICES_def,ROM_DEVICE_def,RAM_DEVICE_def,EMPTY_DEVICE_def,
+    pairTheory.FORALL_PROD,LET_DEF,PERIPHERALS_NEXT_def,FILTER_ACCESSES_def,
+    listTheory.FILTER,ROM_NEXT_def,RAM_NEXT_def,UPDATE_RAM_def,
+    pairTheory.EXISTS_PROD] THEN METIS_TAC [UART0_NEXT_EXISTS]);
+
+
+val _ = export_theory();
