examples/acl2/examples/M1/M1Examples.sml
@@ -1,0 +1,58 @@
+(*****************************************************************************)
+(* Examples of M1                                                            *)
+(*****************************************************************************)
+
+(* Commands when run interactively:
+quietdec := true;                                    (* Switch off output    *)
+
+map load ["sexpTheory","imported_acl2Theory"];
+open sexpTheory imported_acl2Theory;
+
+quietdec := false;                                   (* Restore output       *)
+*)
+
+
+(******************************************************************************
+* Boilerplate needed for compilation: open HOL4 systems modules.
+******************************************************************************)
+open HolKernel Parse boolLib bossLib;
+
+(******************************************************************************
+* Open theories (including ratTheory from Jens Brandt).
+******************************************************************************)
+
+open sexpTheory imported_acl2Theory;
+
+(*****************************************************************************)
+(* END BOILERPLATE                                                           *)
+(*****************************************************************************)
+
+(******************************************************************************
+* Function to simplify imported ACL2
+******************************************************************************)
+
+val acl2_simp =
+ SIMP_RULE
+  list_ss
+  ([let_simp,andl_fold,itel_fold,itel_append,
+    forall2_thm,exists2_thm,forall_fold,exists_fold,
+    implies,andl_simp,not_simp,t_nil]
+   @
+   (map GSYM [int_def,nat_def,List_def,asym_def,csym_def,ksym_def,osym_def]));
+
+(******************************************************************************
+M1 contains simplified definitions and theorems from other theories
+******************************************************************************)
+
+val Examples1 =
+ [("exclaim_def",         acl2_simp exclaim_defun),
+  ("ifact_def",           acl2_simp ifact_defun),
+  ("ifact_lemma",         acl2_simp ifact_lemma_thm),
+  ("ifact_is_factorial",  acl2_simp ifact_is_factorial_thm),
+  ("ifact_correct",       acl2_simp ifact_correct_thm),
+  ("repeat_def",          acl2_simp repeat_defun),
+  ("ifact_sched_def",     acl2_simp ifact_sched_defun),
+  ("test_ifact_examples", acl2_simp test_ifact_examples_thm)];
+
+val Examples2 = map (I ## acl2_simp) (theorems "imported_acl2");
+
