examples/acl2/examples/M1/M1Script.sml
@@ -1,0 +1,74 @@
+(*****************************************************************************)
+(* Create "M1Theory"                                                         *)
+(*****************************************************************************)
+
+(* Commands when run interactively:
+quietdec := true;                                    (* Switch off output    *)
+
+map load ["imported_acl2Theory"];
+open imported_acl2Theory;
+
+quietdec := false;                                   (* Restore output       *)
+*)
+
+
+(******************************************************************************
+* Boilerplate needed for compilation: open HOL4 systems modules.
+******************************************************************************)
+open HolKernel Parse boolLib bossLib;
+
+(******************************************************************************
+* Open theories (including ratTheory from Jens Brandt).
+******************************************************************************)
+
+open stringLib complex_rationalTheory acl2_packageTheory sexp sexpTheory
+     imported_acl2Theory;
+
+(*****************************************************************************)
+(* END BOILERPLATE                                                           *)
+(*****************************************************************************)
+
+(******************************************************************************
+* Start a new theory called M1
+******************************************************************************)
+
+val _ = new_theory "M1";
+
+val simp_fn =
+ SIMP_RULE
+  list_ss
+  ([let_simp,andl_fold,itel_fold,itel_append,
+    forall2_thm,exists2_thm,forall_fold,exists_fold,
+    implies,andl_simp,not_simp,t_nil]
+   @
+   (map GSYM [int_def,nat_def,List_def,asym_def,csym_def,ksym_def,osym_def]));
+
+(******************************************************************************
+M1 contains simplified definitions and theorems from other theories
+******************************************************************************)
+
+val exclaim_def =
+ save_thm("exclaim_def", simp_fn exclaim_defun);
+
+val ifact_def =
+ save_thm("ifact_def", simp_fn ifact_defun);
+
+val ifact_lemma =
+ save_thm("ifact_lemma", simp_fn ifact_lemma_thm);
+
+val ifact_is_factorial =
+ save_thm("ifact_is_factorial", simp_fn ifact_is_factorial_thm);
+
+val ifact_correct =
+ save_thm("ifact_correct", simp_fn ifact_correct_thm);
+
+val repeat_def =
+ save_thm("repeat_def", simp_fn repeat_defun);
+
+val ifact_sched_def =
+ save_thm("ifact_sched_def", simp_fn ifact_sched_defun);
+
+val test_ifact_examples =
+ save_thm("test_ifact_examples", simp_fn test_ifact_examples_thm);
+
+val _ = export_theory();
