examples/acl2/examples/M1/acl2_packageScript.sml
@@ -1,0 +1,201 @@
+(*****************************************************************************)
+(* Defines the list of triples ACL2_PACKAGE_ALIST representing the           *)
+(* initial ACL2 package structure.                                           *)
+(*                                                                           *)
+(* Also defines a predicate VALID_PKG_TRIPLES from Matt Kaufmann that        *)
+(* abstracts key properties of the package structure and verifies:           *)
+(*                                                                           *)
+(*  |- VALID_PKG_TRIPLES  ACL2_PACKAGE_ALIST                                 *)
+(*                                                                           *)
+(* Modified again to split into 4 equal length lists, hence O(n. log n)      *)
+(*                                                                           *)
+(*****************************************************************************)
+
+(*****************************************************************************)
+(* Ignore everything up to "END BOILERPLATE"                                 *)
+(*****************************************************************************)
+
+(*****************************************************************************)
+(* START BOILERPLATE NEEDED FOR COMPILATION                                  *)
+(*****************************************************************************)
+
+(******************************************************************************
+* Load theories
+******************************************************************************)
+(* The commented out stuff below should be loaded in interactive sessions
+quietdec := true;
+map load ["stringLib","pairSyntax","listSyntax","PKGS"];
+open stringLib pairSyntax listSyntax;
+Globals.checking_const_names := false;
+quietdec := false;
+*)
+
+(******************************************************************************
+* Boilerplate needed for compilation: open HOL4 systems modules.
+******************************************************************************)
+
+open HolKernel Parse boolLib bossLib;
+
+(******************************************************************************
+* Open theories (including ratTheory from Jens Brandt).
+******************************************************************************)
+
+open listSyntax pairSyntax stringLib listTheory;
+
+(*****************************************************************************)
+(* END BOILERPLATE                                                           *)
+(*****************************************************************************)
+
+(*****************************************************************************)
+(* Start new theory "acl2_package"                                           *)
+(*****************************************************************************)
+val _ = new_theory "acl2_package";
+
+(*****************************************************************************)
+(* ACL2_PACKAGE_ALIST contains a list of triples                             *)
+(*                                                                           *)
+(*   (symbol-name , known-pkg-name , actual-pkg-name)                        *)
+(*                                                                           *)
+(* The idea is that when symbol-name is interned into known-pkg-name, the    *)
+(* resulting symbol's package name is actual-pkg-name.  That is, the         *)
+(* symbol with name symbol-name and package-name actual-pkg-name is          *)
+(* imported into package known-pkg-name.                                     *)
+(*****************************************************************************)
+
+
+(*****************************************************************************)
+(* Building a term directly out of a slurped in ACL2 package structure       *)
+(* (e.g. kpa-v2-9-3.ml) breaks the HOL compiler. We therefore fold in the    *)
+(* abbreviations below (this idea due to Konrad). It is strange that         *)
+(* rewriting the big term is no problem, but compiling it breaks.            *)
+(*****************************************************************************)
+val ACL2_CL_def     = Define `ACL2_CL      = ("ACL2", "COMMON-LISP")`;
+val ACL2_USER_def   = Define `ACL2_USER    = ("ACL2-USER" , "ACL2")`;
+val ACL_USER_CL_def = Define `ACL2_USER_CL = ("ACL2-USER" , "COMMON-LISP")`;
+
+(*****************************************************************************)
+(* Convert imported ACL2 package structure:                                  *)
+(*                                                                           *)
+(*  [                                                                        *)
+(*  ("&", "ACL2-USER", "ACL2"),                                              *)
+(*  ("*ACL2-EXPORTS*", "ACL2-USER", "ACL2"),                                 *)
+(*  ...                                                                      *)
+(*  ("VALUES", "ACL2", "COMMON-LISP"),                                       *)
+(*  ("ZEROP", "ACL2", "COMMON-LISP")                                         *)
+(*  ]                                                                        *)
+(*                                                                           *)
+(* to corresponding term, then fold in ACL2_CL_def, ACL2_USER_def and        *)
+(* ACL_USER_CL_def using REWRITE_CONV, then extract the simplified term.     *)
+(* Used to define ACL2_PACKAGE_ALIST                                         *)
+(*****************************************************************************)
+
+fun make_package_structure_term l =
+ rhs
+  (concl
+    (REWRITE_CONV
+      (map GSYM [ACL2_CL_def,ACL2_USER_def,ACL_USER_CL_def])
+      (mk_list
+       (map
+         (fn (s1,s2,s3) =>
+           mk_pair(fromMLstring s1, mk_pair(fromMLstring s2, fromMLstring s3)))
+        l,
+        ``:string # string # string``))));
+
+(*****************************************************************************)
+(* The actual triples specifying the initial ACL2 package                    *)
+(*****************************************************************************)
+val ACL2_PACKAGE_ALIST_def =
+ time
+  Define
+  `ACL2_PACKAGE_ALIST =
+    ^(make_package_structure_term PKGS.ACL2_PACKAGE_ALIST)`;
+
+val ACL2_KNOWN_PACKAGES_def =
+ time
+  Define
+  `ACL2_KNOWN_PACKAGES =
+    ^(listSyntax.mk_list
+       (map fromMLstring PKGS.ACL2_KNOWN_PACKAGES,
+        ``:string``))`;
+
+(*****************************************************************************)
+(* (defun lookup (pkg-name triples sym-name)                                 *)
+(*                                                                           *)
+(* ; Triples is a list of "package triples" of the form (sym-name            *)
+(* ; pkg-name orig-pkg-name) representing that the symbol-package-name of    *)
+(* ; pkg-name::sym-anme is orig-pkg-name.  Lookup returns the                *)
+(* ; symbol-package-name of pkg-name::sym-name.                              *)
+(*                                                                           *)
+(*   (cond ((endp triples)                                                   *)
+(*          pkg-name)                                                        *)
+(*         ((and (equal pkg-name (nth 1 (car triples)))                      *)
+(*               (equal sym-name (nth 0 (car triples))))                     *)
+(*          (nth 2 (car triples)))                                           *)
+(*         (t (lookup pkg-name (cdr triples) sym-name))))                    *)
+(*                                                                           *)
+(* LOOKUP pkg_name [(x1,y1,z1);...;(xn,yn,zn)] sym_name  =  zi               *)
+(*    if for some i: sym_name=xi and pkg_name=yi (scanning from left)        *)
+(*                                                                           *)
+(* LOOKUP pkg_name [(x1,y1,z1);...;(xn,yn,zn)] sym_name  =  pkg_name         *)
+(*    if for all i: ~(sym_name=xi and pkg_name=yi)                           *)
+(*                                                                           *)
+(*****************************************************************************)
+val LOOKUP_def =
+ Define
+  `(LOOKUP pkg_name [] _ = pkg_name) 
+   /\
+   (LOOKUP pkg_name ((x1,y1,z1)::a) sym_name = 
+     if (sym_name=x1) /\ (pkg_name=y1) 
+       then z1 
+       else LOOKUP pkg_name a sym_name)`;
+
+(*****************************************************************************)
+(* (defun valid-pkg-triples-aux (tail triples)                               *)
+(*                                                                           *)
+(* ; We recognize whether tail, a tail of triples, is a legal list of        *)
+(* ; package triples with respect to the full list, triples.  The idea is    *)
+(* ; that for any symbol s imported from package p1 to package p2, s         *)
+(* ; cannot be imported from some other package p0 into p1.  That is,        *)
+(* ; lookup is idempotent.                                                   *)
+(*                                                                           *)
+(*   (if (endp tail)                                                         *)
+(*       t                                                                   *)
+(*     (let* ((trip (car tail))                                              *)
+(*            (sym-name (nth 0 trip))                                        *)
+(*            (p2 (nth 2 trip)))                                             *)
+(*         (and (equal (lookup p2 triples sym-name)                          *)
+(*                     p2)                                                   *)
+(*              (not (equal sym-name "ACL2-PKG-WITNESS"))                    *)
+(*              (not (equal p2 ""))                                          *)
+(*              (valid-pkg-triples-aux (cdr tail) triples)))))               *)
+(*****************************************************************************)
+val VALID_PKG_TRIPLES_AUX_def =
+ Define
+  `(VALID_PKG_TRIPLES_AUX [] triples = T)
+   /\
+   (VALID_PKG_TRIPLES_AUX ((sym_name,_,p2)::tail) triples =
+     (LOOKUP p2 triples sym_name = p2) /\
+     ~(sym_name = "ACL2-PKG-WITNESS")  /\
+     ~(p2 = "")                        /\
+     (VALID_PKG_TRIPLES_AUX tail triples))`;
+
+val VALID_PKG_TRIPLES_def =
+ Define
+  `VALID_PKG_TRIPLES triples = VALID_PKG_TRIPLES_AUX triples triples`;
+
+
+(*
+
+val VALID_ACL2_PACKAGE_ALIST = 
+ save_thm
+  ("VALID_ACL2_PACKAGE_ALIST",
+   Count.apply (time EVAL) ``VALID_PKG_TRIPLES ACL2_PACKAGE_ALIST``);
+
+This causes an overflow:
+
+  OverflowUncaught exception:
+  Overflow
+
+*)
+
+val _ = export_theory();
