examples/acl2/ml/signedintScript.sml
@@ -1508,7 +1508,7 @@ val WORD_BITS_THM = store_thm("WORD_BITS_THM",
     RW_TAC int_ss [fcpTheory.CART_EQ,fcpTheory.FCP_BETA,word_bits_def,
     	   word_and_def,word_lsr_def,
 	   PROVE [word_index_n2w] ``i < dimindex (:'a) ==>
-	   	 (n2w n : 'a word ' i = BIT i n)``,word_asr_def,
+	   	 ((n2w n :'a word) ' i = BIT i n)``,word_asr_def,
 	   BIT_RANGE,TOP_BIT_THM] THEN EQ_TAC THEN
     RW_TAC int_ss [DECIDE ``i < a + 1 - b = i + b <= a:num``]);
 
@@ -1517,7 +1517,7 @@ val WORD_SLICE_THM = store_thm("WORD_SLICE_THM",
     RW_TAC int_ss [fcpTheory.CART_EQ,fcpTheory.FCP_BETA,word_bits_def,
     	   word_and_def,word_lsr_def,
 	   PROVE [word_index_n2w] 
-             ``i < dimindex (:'a) ==> (n2w n : 'a word ' i = BIT i n)``, 
+             ``i < dimindex (:'a) ==> ((n2w n :'a word) ' i = BIT i n)``, 
             word_asr_def, BIT_RANGE,TOP_BIT_THM,word_slice_def] THEN
     EQ_TAC THEN RW_TAC int_ss []);
 
