src/datatype/selftest.sml
@@ -155,6 +155,22 @@ val result = ind_types.define_type spec' handle e => Raise e;
 
 *)
 
+(* Ramana Kumar's example from 2010/08/19 *)
+val _ = Hol_datatype`pointer = pnil | pref of 'a`
+val _ = Hol_datatype`failure = <| head : 'a pointer; tail : failure pointer |>`
+
+(* Ramana Kumar's examples from 2010/08/25 *)
+val _ = Hol_datatype `t1 = c1 of 'a => t1 itself `;
+val _ = Hol_datatype `t2 = c2 of t2 t1 itself ` ;
+
+val _ = Hol_datatype `u1 = d1 of 'a itself`;
+val _ = Hol_datatype `u2 = d2 of 'a u1 `;
+val _ = Hol_datatype `u3 = d3 of u4 u2 u1 ;
+                      u4 = d4 of u3 u1 `;
+
+(* Ramana Kumar's TypeNet bug from 2010/08/25 *)
+val _ = Hol_datatype `foo = fooC of 'a`
+val _ = Hol_datatype `foo = fooC' of num`
 
 fun tprint s = print (StringCvt.padRight #" " 70 s)
 
