src/list/src/listScript.sml
@@ -966,6 +966,47 @@ REWRITE_TAC[relationTheory.WF_DEF] THEN BETA_TAC THEN GEN_TAC
   THENL [FIRST_ASSUM ACCEPT_TAC,
          PAT_ASSUM (Term`x /\ y`) (SUBST_ALL_TAC o CONJUNCT2) THEN RES_TAC]);
 
+(* ----------------------------------------------------------------------
+    LIST_REL : ('a -> 'b -> bool) -> 'a list -> 'b list -> bool
+
+    Lifts a relation point-wise to two lists
+   ---------------------------------------------------------------------- *)
+
+val (LIST_REL_rules, LIST_REL_ind, LIST_REL_cases) = IndDefLib.Hol_reln`
+  (LIST_REL R [] []) /\
+  (!h1 h2 t1 t2. R h1 h2 /\ LIST_REL R t1 t2 ==> LIST_REL R (h1::t1) (h2::t2))
+`;
+
+val LIST_REL_EL_EQN = store_thm(
+  "LIST_REL_EL_EQN",
+  ``!R l1 l2. LIST_REL R l1 l2 <=>
+              (LENGTH l1 = LENGTH l2) /\
+              !n. n < LENGTH l1 ==> R (EL n l1) (EL n l2)``,
+  GEN_TAC THEN SIMP_TAC (srw_ss()) [EQ_IMP_THM, FORALL_AND_THM] THEN
+  CONJ_TAC THENL [
+    Induct_on `LIST_REL` THEN SRW_TAC [][] THEN
+    Cases_on `n` THEN FULL_SIMP_TAC (srw_ss()) [],
+    Induct_on `l1` THEN Cases_on `l2` THEN SRW_TAC [][LIST_REL_rules] THEN
+    POP_ASSUM (fn th => Q.SPEC_THEN `0` MP_TAC th THEN
+                        Q.SPEC_THEN `SUC m` (MP_TAC o Q.GEN `m`) th) THEN
+    SRW_TAC [][LIST_REL_rules]
+  ]);
+
+val LIST_REL_def = store_thm(
+  "LIST_REL_def",
+  ``(LIST_REL R [][] <=> T) /\
+    (LIST_REL R (a::as) [] <=> F) /\
+    (LIST_REL R [] (b::bs) <=> F) /\
+    (LIST_REL R (a::as) (b::bs) <=> R a b /\ LIST_REL R as bs)``,
+  REPEAT CONJ_TAC THEN SRW_TAC [][Once LIST_REL_cases, SimpLHS]);
+val _ = export_rewrites ["LIST_REL_def"]
+
+val LIST_REL_mono = store_thm(
+  "LIST_REL_mono",
+  ``(!x y. R1 x y ==> R2 x y) ==> LIST_REL R1 l1 l2 ==> LIST_REL R2 l1 l2``,
+  SRW_TAC [][LIST_REL_EL_EQN]);
+val _ = IndDefLib.export_mono "LIST_REL_mono"
+
 (*---------------------------------------------------------------------------
      Congruence rules for higher-order functions. Used when making
      recursive definitions by so-called higher-order recursion.
@@ -1262,6 +1303,13 @@ val MEM_EL = store_thm(
     Cases_on `n` THEN FULL_SIMP_TAC arith_ss [EL, HD, TL] THEN
     ASM_MESON_TAC []
   ]);
+
+val SUM_MAP_PLUS_ZIP = store_thm(
+  "SUM_MAP_PLUS_ZIP",
+  ``!ls1 ls2. (LENGTH ls1 = LENGTH ls2) /\ (!x y. f (x,y) = g x + h y) ==>
+              (SUM (MAP f (ZIP (ls1,ls2))) = SUM (MAP g ls1) + SUM (MAP h ls2))``,
+  Induct THEN Cases_on `ls2` THEN
+  SRW_TAC [numSimps.ARITH_ss][MAP,ZIP,MAP_ZIP,SUM]);
 
 (* --------------------------------------------------------------------- *)
 (* REVERSE                                                               *)
@@ -1644,6 +1692,13 @@ val FINITE_LIST_TO_SET = Q.store_thm
  Induct THEN SRW_TAC [][]);
 val _ = export_rewrites ["FINITE_LIST_TO_SET"]
 
+val SUM_IMAGE_LIST_TO_SET_upper_bound = store_thm(
+  "SUM_IMAGE_LIST_TO_SET_upper_bound",
+  ``!ls. SIGMA f (set ls) <= SUM (MAP f ls)``,
+  Induct THEN
+  SRW_TAC [][MAP,SUM,SUM_IMAGE_THM,SUM_IMAGE_DELETE] THEN
+  numLib.DECIDE_TAC);
+
 local open numLib in
 val CARD_LIST_TO_SET = Q.store_thm(
 "CARD_LIST_TO_SET",
@@ -1668,6 +1723,11 @@ val LIST_TO_SET_MAP = store_thm ("LIST_TO_SET_MAP",
 Induct_on `l` THEN
 ASM_SIMP_TAC bool_ss [pred_setTheory.IMAGE_EMPTY, pred_setTheory.IMAGE_INSERT,
    MAP, LIST_TO_SET_THM]);
+
+val LIST_TO_SET_FILTER = store_thm(
+  "LIST_TO_SET_FILTER",
+  ``LIST_TO_SET (FILTER P l) = { x | P x } INTER LIST_TO_SET l``,
+  SRW_TAC [][pred_setTheory.EXTENSION, MEM_FILTER]);
 
 
 (* ----------------------------------------------------------------------
